src/Pipit.Exp.Binding.Properties.fst
@@ -48,7 +48,7 @@ let rec lemma_lift_lift_commute (e: exp 'c 'a) (i1: C.index { i1 <= List.Tot.len
     lemma_lift_lift_commute e1 i1 i2 t1 t2;
     lemma_lift_lift_commute e2 i1 i2 t1 t2
 
-let rec lemma_subst_lift_id (e: exp 'c 'a) (i: C.index { C.has_index 'c i }) (t: Type) (p: exp 'c t):
+let rec lemma_subst_lift_id (e: exp 'c 'a) (i: C.index { i <= List.Tot.length 'c }) (t: Type) (p: exp 'c t):
   Lemma (ensures (
     subst1' (lift1' e i t) i p == e))
     (decreases e) =
@@ -169,38 +169,64 @@ let rec lemma_lift_subst_distribute_le (e: exp 'c 'a) (i1: C.index { C.has_index
     lemma_lift_subst_distribute_le e2 i1 i2 t2 p;
     ()
 
-let rec lemma_subst_subst_distribute_le (e: exp 'c 'a) (i1: C.index { C.has_index 'c i1 }) (i2: C.index { i1 <= i2 /\ i2 < List.Tot.length 'c - 1 }) (p1: exp (C.drop1 'c i1) (C.get_index 'c i1)) (p2: exp (C.drop1 (C.drop1 'c i1) i2) (C.get_index (C.drop1 'c i1) i2)):
+let lemma_subst_subst_distribute_le_base (e: base_exp 'c 'a) (i1: C.index { C.has_index 'c i1 }) (i2: C.index { i1 <= i2 /\ i2 < List.Tot.length 'c - 1 }) (p1: exp (C.drop1 'c i1) (C.get_index 'c i1)) (p2: exp (C.drop1 (C.drop1 'c i1) i2) (C.get_index (C.drop1 'c i1) i2)):
   Lemma (ensures
-    C.lemma_lift_drop_commute_le (C.drop1 'c i1) i2 i1 (C.get_index 'c i1);
     C.lemma_drop_drop_commute 'c i1 i2;
-    C.lemma_lift_drop_eq 'c i1;
-    C.lemma_drop_get_index_gt 'c i1 i2;
     C.lemma_drop_get_index_lt 'c (i2 + 1) i1;
-    // let p2': exp (C.drop1 (C.lift1 (C.drop1 'c i1) i1 (C.get_index 'c i1)) (i2 + 1)) (C.get_index (C.drop1 'c i1) i2) = lift1' p2 i1 (C.get_index 'c i1) in
-    // let p2': exp (C.drop1 'c (i2 + 1)) (C.get_index (C.drop1 'c i1) i2) = p2' in
-    // let p2': exp (C.drop1 'c (i2 + 1)) (C.get_index 'c (i2 + 1)) = p2' in
     subst1' (subst1' e i1 p1) i2 p2 ==
     subst1' (subst1' e (i2 + 1) (lift1' p2 i1 (C.get_index 'c i1))) i1 (subst1' p1 i2 p2)) =
-  C.lemma_lift_drop_commute_le (C.drop1 'c i1) i2 i1 (C.get_index 'c i1);
   C.lemma_drop_drop_commute 'c i1 i2;
-  C.lemma_lift_drop_eq 'c i1;
-  C.lemma_drop_get_index_gt 'c i1 i2;
   C.lemma_drop_get_index_lt 'c (i2 + 1) i1;
   match e with
   | XVal v -> ()
   | XVar _ -> ()
   | XBVar i' ->
-    // if i' = i2 + 1
-    // then lemma_subst_lift_id p2 i1 (C.get_index 'c i1) (subst1' p1 i2 p2)
-    admit ()
+    if i' = i1
+    then ()
+    else if i' = i2 + 1
+    then begin
+      calc (==) {
+        C.lift1 (C.drop1 (C.drop1 'c i1) i2) i1 (C.get_index 'c i1);
+        (==) { C.lemma_lift_drop_commute_le (C.drop1 'c i1) i2 i1 (C.get_index 'c i1) }
+        C.drop1 (C.lift1 (C.drop1 'c i1) i1 (C.get_index 'c i1)) (i2 + 1);
+        (==) { C.lemma_lift_drop_eq 'c i1 }
+        C.drop1 'c (i2 + 1);
+      };
+      let p2': exp (C.drop1 'c (i2 + 1)) (C.get_index (C.drop1 'c i1) i2) = coerce_eq () (lift1' p2 i1 (C.get_index 'c i1)) in
+      calc (==) {
+        subst1' (subst1' e (i2 + 1) p2') i1 (subst1' p1 i2 p2);
+        (==) { }
+        subst1' (lift1' p2 i1 (C.get_index 'c i1)) i1 (subst1' p1 i2 p2);
+        (==) { lemma_subst_lift_id p2 i1 (C.get_index 'c i1) (subst1' p1 i2 p2) }
+        p2;
+      };
+      ()
+    end
+    else ()
+
+let rec lemma_subst_subst_distribute_le (e: exp 'c 'a) (i1: C.index { C.has_index 'c i1 }) (i2: C.index { i1 <= i2 /\ i2 < List.Tot.length 'c - 1 }) (p1: exp (C.drop1 'c i1) (C.get_index 'c i1)) (p2: exp (C.drop1 (C.drop1 'c i1) i2) (C.get_index (C.drop1 'c i1) i2)):
+  Lemma (ensures
+    (C.lemma_drop_drop_commute 'c i1 i2;
+    C.lemma_drop_get_index_lt 'c (i2 + 1) i1;
+    subst1' (subst1' e i1 p1) i2 p2 ==
+    subst1' (subst1' e (i2 + 1) (lift1' p2 i1 (C.get_index 'c i1))) i1 (subst1' p1 i2 p2)))
+    (decreases e) =
+  // C.lemma_lift_drop_commute_le (C.drop1 'c i1) i2 i1 (C.get_index 'c i1);
+  C.lemma_drop_drop_commute 'c i1 i2;
+  // C.lemma_lift_drop_eq 'c i1;
+  // C.lemma_drop_get_index_gt 'c i1 i2;
+  C.lemma_drop_get_index_lt 'c (i2 + 1) i1;
+  match e with
+  | XVal _ | XVar _ | XBVar _ -> lemma_subst_subst_distribute_le_base e i1 i2 p1 p2
+
   | XApp e1 e2 ->
     lemma_subst_subst_distribute_le e1 i1 i2 p1 p2;
     lemma_subst_subst_distribute_le e2 i1 i2 p1 p2;
-    // assert_norm (lift1' (subst1' (XApp e1 e2) i1 p) i2 t2 ==
-    //   XApp (lift1' (subst1' e1 i1 p) i2 t2) (lift1' (subst1' e2 i1 p) i2 t2));
-    // assert_norm (subst1' (lift1' (XApp e1 e2) i2 t2) (i1 + 1) (lift1' p i2 t2) ==
-    //   XApp (subst1' (lift1' e1 i2 t2) (i1 + 1) (lift1' p i2 t2)) (subst1' (lift1' e2 i2 t2) (i1 + 1) (lift1' p i2 t2)));
-    admit ()
+    assert_norm (subst1' (subst1' (XApp e1 e2) i1 p1) i2 p2 ==
+      XApp (subst1' (subst1' e1 i1 p1) i2 p2) (subst1' (subst1' e2 i1 p1) i2 p2));
+    assert_norm (subst1' (subst1' (XApp e1 e2) (i2 + 1) (lift1' p2 i1 (C.get_index 'c i1))) i1 (subst1' p1 i2 p2) ==
+      XApp (subst1' (subst1' e1 (i2 + 1) (lift1' p2 i1 (C.get_index 'c i1))) i1 (subst1' p1 i2 p2)) (subst1' (subst1' e2 (i2 + 1) (lift1' p2 i1 (C.get_index 'c i1))) i1 (subst1' p1 i2 p2)));
+    ()
   | XFby v e1 ->
     lemma_subst_subst_distribute_le e1 i1 i2 p1 p2;
     ()
@@ -208,39 +234,54 @@ let rec lemma_subst_subst_distribute_le (e: exp 'c 'a) (i1: C.index { C.has_inde
     lemma_subst_subst_distribute_le e1 i1 i2 p1 p2;
     lemma_subst_subst_distribute_le e2 i1 i2 p1 p2;
     ()
-  | XMu _ e1 ->
-    // C.lemma_lift_drop_commute_le 'c i1 0 'a;
-    // C.lemma_lift_get_index_gt 'c i1 i2 'a;
-    // lemma_lift_lift_commute p i2 0 t2 'a;
-    // let p' = _lift_of_drop i1 p 'a in
-    // lemma_subst_subst_distribute_le e1 (i1 + 1) (i2 + 1) t2 p'
-
-    // lemma_lift_lift_commute p2 x1 0;
-    // lift_subst_distribute_le p1 p2 x2 0
-    admit ()
-
-  | XLet b e1 e2 ->
-    admit ()
-  //   lemma_lift_lift_commute p i2 0 t2 b;
-  //   let p' = _lift_of_drop i1 p b in
-
-  //   C.lemma_lift_get_index_gt 'c i1 0 b;
-  //   C.lemma_lift_get_index_gt (b :: 'c) (i1 + 1) (i2 + 1) t2;
-
-  //   C.lemma_lift_drop_commute_le 'c i1 i2 t2;
-
-  //   lemma_subst_subst_distribute_le e1 i1 i2 t2 p;
-  //   lemma_subst_subst_distribute_le e2 (i1 + 1) (i2 + 1) t2 p';
-
-  //   ()
-    // lemma_lift_lift_commute p2 x1 0;
-    // lift_subst_distribute_le p1 p2 x2 0
-
   | XCheck _ e1 e2 ->
     lemma_subst_subst_distribute_le e1 i1 i2 p1 p2;
     lemma_subst_subst_distribute_le e2 i1 i2 p1 p2;
     ()
-// TODO prove it
+
+  | XMu _ e1 ->
+    let p1' = _lift_of_drop i1 p1 'a in
+    let p2' = _lift_of_drop i2 p2 'a in
+    lemma_subst_subst_distribute_le e1 (i1 + 1) (i2 + 1) p1' p2';
+    lemma_lift_lift_commute p2 i1 0 (C.get_index 'c i1) 'a;
+    lemma_lift_subst_distribute_le p1 i2 0 'a p2;
+
+    C.lemma_lift_drop_commute_le (C.drop1 'c i1) i2 i1 (C.get_index 'c i1);
+    C.lemma_lift_drop_eq 'c i1;
+
+    // assert (C.get_index ('a :: 'c) (i1 + 1) == C.get_index 'c i1);
+    // assert (subst1' (subst1' (XMu e1) i1 p1) i2 p2 ==
+    //   XMu (subst1' (subst1' e1 (i1 + 1) p1') (i2 + 1) p2'));
+
+    // assert ('a :: C.drop1 (C.drop1 'c (i2 + 1)) i1 == C.drop1 (C.drop1 ('a :: 'c) (i2 + 2)) (i1 + 1));
+    // assert (C.get_index ('a :: 'c) (i2 + 2) == C.get_index ('a :: C.drop1 'c i1) (i2 + 1));
+    // assert (C.drop1 ('a :: 'c) (i2 + 2) == C.lift1 (C.drop1 ('a :: C.drop1 'c i1) (i2 + 1)) (i1 + 1) (C.get_index 'c i1));
+
+    // assert (subst1' (subst1' (XMu e1) (i2 + 1) (lift1' p2 i1 (C.get_index 'c i1))) i1 (subst1' p1 i2 p2) ==
+    //   XMu (subst1' (subst1' e1 (i2 + 2) (lift1' p2' (i1 + 1) (C.get_index 'c i1))) (i1 + 1) (subst1' p1' (i2 + 1) p2')));
+
+    // assert (
+    //   (subst1' (subst1' e1 (i1 + 1) p1') (i2 + 1) p2') ==
+    //   (subst1' (subst1' e1 (i2 + 2) (lift1' p2' (i1 + 1) (C.get_index ('a :: 'c) (i1 + 1)))) (i1 + 1) (subst1' p1' (i2 + 1) p2')));
+    // ()
+    admit ()
+  | XLet b e1 e2 ->
+    admit ()
+//   | XLet b e1 e2 ->
+//   //   lemma_lift_lift_commute p i2 0 t2 b;
+//   //   let p' = _lift_of_drop i1 p b in
+
+//   //   C.lemma_lift_get_index_gt 'c i1 0 b;
+//   //   C.lemma_lift_get_index_gt (b :: 'c) (i1 + 1) (i2 + 1) t2;
+
+//   //   C.lemma_lift_drop_commute_le 'c i1 i2 t2;
+
+//   //   lemma_subst_subst_distribute_le e1 i1 i2 t2 p;
+//   //   lemma_subst_subst_distribute_le e2 (i1 + 1) (i2 + 1) t2 p';
+
+//   //   ()
+//     // lemma_lift_lift_commute p2 x1 0;
+//     // lift_subst_distribute_le p1 p2 x2 0
 
 let lemma_subst_subst_distribute_XMu {| Pipit.Inhabited.inhabited 'a |} (e: exp ('a :: 'c) 'a) (i: C.index { C.has_index 'c i }) (p: exp (C.drop1 'c i) (C.get_index 'c i)):
   Lemma (ensures
